Major mostly cosmetic changes

src/verify.lean
@@ -5,75 +5,75 @@ import data.list.alist
 import data.finsupp.basic
 import control.bifunctor
 import finsupp_lemmas
+import frames
 
+section
 -- This is just some experiments I'm doing, unofficial
 -- Anything that works out will go back into compile.lean
 
-variables (R : Type) [add_zero_class R] [has_one R] [has_mul R]
-
+parameters {R : Type} [add_zero_class R] [has_one R] [has_mul R]
+parameter (R)
 -- Same thing as `ℕ ⊕ R` TODO: change or keep?
 inductive ExprVal
 | nat (n : ℕ)
 | rval (r : R)
 
+parameter {R}
 namespace ExprVal
-variable {R}
+instance : inhabited ExprVal := ⟨nat 0⟩
 
-instance : inhabited (ExprVal R) := ⟨nat 0⟩
-
-instance [has_repr R] : has_repr (ExprVal R) :=
+instance [has_repr R] : has_repr ExprVal :=
 ⟨λ v, match v with
 | (nat n) := "(nat " ++ (repr n) ++ ")"
 | (rval r) := "(rval " ++ (repr r) ++ ")"
 end⟩
 
 @[simp]
-def add : ExprVal R → ExprVal R → ExprVal R
+def add : ExprVal → ExprVal → ExprVal
 | (nat n₁) (nat n₂) := nat (n₁ + n₂)
 | (rval f₁) (rval f₂) := rval (f₁ + f₂)
 | _ _ := arbitrary _
 
 @[simp]
-def and : ExprVal R → ExprVal R → ExprVal R
+def and : ExprVal → ExprVal → ExprVal
 | (nat n₁) (nat n₂) := if n₁ = 0 then nat 0 else nat n₂
 | _ _ := arbitrary _
 
 @[simp]
-def mul : ExprVal R → ExprVal R → ExprVal R
+def mul : ExprVal → ExprVal → ExprVal
 | (nat n₁) (nat n₂) := nat (n₁ * n₂)
 | (rval f₁) (rval f₂) := rval (f₁ * f₂)
 | _ _ := arbitrary _
 
 @[simp]
-def not : ExprVal R → ExprVal R
+def not : ExprVal → ExprVal
 | (nat n₁) := if n₁ = 0 then nat 1 else nat 0
 | _ := arbitrary _
 
 @[simp]
-def to_nat : ExprVal R → ℕ
+def to_nat : ExprVal → ℕ
 | (nat n₁) := n₁
 | _ := default
 
 @[simp]
-def eq : ExprVal R → ExprVal R → ExprVal R
+def eq : ExprVal → ExprVal → ExprVal
 | (nat n₁) (nat n₂) := if n₁ = n₂ then nat 1 else nat 0
 | _ _ := arbitrary _
 
 @[simp]
-def lt : ExprVal R → ExprVal R → ExprVal R
+def lt : ExprVal → ExprVal → ExprVal
 | (nat n₁) (nat n₂) := if n₁ < n₂ then nat 1 else nat 0
 | _ _ := arbitrary _
 
 @[simp]
-def to_r : ExprVal R → R
+def to_r : ExprVal → R
 | (nat n) := n
 | (rval r) := r
 
 @[simp]
-def cast_r (v : ExprVal R) : ExprVal R := rval v.to_r
+def cast_r (v : ExprVal) : ExprVal := rval v.to_r
 
 end ExprVal
-
 section Ident
 
 
@@ -92,29 +92,30 @@ instance : has_repr Ident := ⟨λ i, match i with
 | (Ident.num n) := "x" ++ (repr n)
 end⟩
 
+parameter (R)
 inductive IdentVal
-| base (val : ExprVal R) : IdentVal
-| arr (val : list (ExprVal R)) : IdentVal
-instance : inhabited (IdentVal R) := ⟨IdentVal.base default⟩ 
+| base (val : ExprVal) : IdentVal
+| arr (val : list (ExprVal)) : IdentVal
+instance : inhabited IdentVal := ⟨IdentVal.base default⟩ 
 
-variable {R}
-def IdentVal.get : IdentVal R → option ℕ → ExprVal R
+parameter {R}
+def IdentVal.get : IdentVal → option ℕ → ExprVal
 | (IdentVal.base val) none := val
 | (IdentVal.arr val) (some i) := val.inth i
 | _ _ := arbitrary _ 
 
-@[simp] lemma IdentVal.get_none (b : ExprVal R) : (IdentVal.base b).get none = b := rfl
-@[simp] lemma IdentVal.get_ind (arr : list (ExprVal R)) (n : ℕ) :
+@[simp] lemma IdentVal.get_none (b : ExprVal) : (IdentVal.base b).get none = b := rfl
+@[simp] lemma IdentVal.get_ind (arr : list ExprVal) (n : ℕ) :
   (IdentVal.arr arr).get (some n) = arr.inth n := rfl
 
-def IdentVal.update : IdentVal R → option ℕ → ExprVal R → IdentVal R
+def IdentVal.update : IdentVal → option ℕ → ExprVal → IdentVal
 | (IdentVal.arr val) (some i) newval := IdentVal.arr (val.modify_nth (λ _, newval) i)
 | _ none newval := IdentVal.base newval
 | _ _ _ := arbitrary _
 
-@[simp] lemma IdentVal.update_none (i : IdentVal R) (x : ExprVal R) :
+@[simp] lemma IdentVal.update_none (i : IdentVal) (x : ExprVal) :
   i.update none x = IdentVal.base x := by cases i; simp [IdentVal.update]
-@[simp] lemma IdentVal.update_ind (arr : list (ExprVal R)) (n : ℕ) (x : ExprVal R) :
+@[simp] lemma IdentVal.update_ind (arr : list ExprVal) (n : ℕ) (x : ExprVal) :
   (IdentVal.arr arr).update (some n) x = IdentVal.arr (arr.modify_nth (λ _, x) n) := rfl
 
 end Ident
@@ -145,9 +146,8 @@ end⟩
 | Op.lt := 2
 | Op.cast_r := 1
 
-variable {R}
 @[simp]
-def eval : ∀ o : Op, (fin o.arity → ExprVal R) → ExprVal R
+def eval : ∀ o : Op, (fin o.arity → ExprVal) → ExprVal
 | add := λ x, (x 0).add (x 1)
 | mul := λ x, (x 0).mul (x 1)
 | and := λ x, (x 0).and (x 1)
@@ -158,44 +158,43 @@ def eval : ∀ o : Op, (fin o.arity → ExprVal R) → ExprVal R
 | cast_r := λ x, (x 0).cast_r
 end Op
 
-variable (R)
+parameter (R)
 inductive Expr
-| lit : ExprVal R → Expr
+| lit : ExprVal → Expr
 | ident : Ident → Expr
 | access : Ident → Expr → Expr
 | call : ∀ o : Op, (fin o.arity → Expr) → Expr
 
-notation a ` ⟪+⟫ `:80 b := Expr.call Op.add ![a, b]
-notation a ` ⟪*⟫ `:80 b := Expr.call Op.mul ![a, b]
-notation a ` ⟪&&⟫ `:80 b := Expr.call Op.and ![a, b]
-notation a ` ⟪||⟫ `:80 b := Expr.call Op.or ![a, b]
-notation a ` ⟪<⟫ `:80 b := Expr.call Op.lt ![a, b]
-notation a ` ⟪=⟫ `:80 b := Expr.call Op.eq ![a, b]
-
-variable {R}
+parameter {R}
+local notation a ` ⟪+⟫ `:80 b := Expr.call Op.add ![a, b]
+local notation a ` ⟪*⟫ `:80 b := Expr.call Op.mul ![a, b]
+local notation a ` ⟪&&⟫ `:80 b := Expr.call Op.and ![a, b]
+local notation a ` ⟪||⟫ `:80 b := Expr.call Op.or ![a, b]
+local notation a ` ⟪<⟫ `:80 b := Expr.call Op.lt ![a, b]
+local notation a ` ⟪=⟫ `:80 b := Expr.call Op.eq ![a, b]
 
 @[simp]
-def Expr.eval  (ctx : Ident → IdentVal R) : Expr R → ExprVal R
+def Expr.eval  (ctx : Ident → IdentVal) : Expr → ExprVal
 | (Expr.lit r) := r
 | (Expr.ident x) := (ctx x).get none
 | (Expr.access x i) := (ctx x).get (some i.eval.to_nat)
 | (Expr.call o args) := o.eval (λ i, (args i).eval)
 
-instance has_coe_from_nat : has_coe ℕ (Expr R) := ⟨λ n, Expr.lit $ ExprVal.nat n⟩
-instance has_coe_From_R : has_coe R (Expr R) := ⟨λ r, Expr.lit $ ExprVal.rval r⟩
-instance has_coe_from_expr : has_coe Ident (Expr R) := ⟨Expr.ident⟩
+instance has_coe_from_nat : has_coe ℕ Expr := ⟨λ n, Expr.lit $ ExprVal.nat n⟩
+instance has_coe_From_R : has_coe R Expr := ⟨λ r, Expr.lit $ ExprVal.rval r⟩
+instance has_coe_from_expr : has_coe Ident Expr := ⟨Expr.ident⟩
 
-example : Expr R := (0 : ℕ)
-example : Expr R := (0 : R)
+example : Expr := (0 : ℕ)
+example : Expr := (0 : R)
 
-@[simp] lemma Expr.eval_const_nat (ctx : Ident → IdentVal R) (n : ℕ) :
+@[simp] lemma Expr.eval_const_nat (ctx : Ident → IdentVal) (n : ℕ) :
   Expr.eval ctx n = ExprVal.nat n := rfl
 
-@[simp] lemma Expr.eval_const_r (ctx : Ident → IdentVal R) (r : R) :
+@[simp] lemma Expr.eval_const_r (ctx : Ident → IdentVal) (r : R) :
   Expr.eval ctx r = ExprVal.rval r := rfl
 
-@[simp] lemma Expr.eval_coe_ident (ctx : Ident → IdentVal R) (i : Ident) :
-  Expr.eval ctx i = (ctx i).get none := rfl 
+@[simp] lemma Expr.eval_coe_ident (ctx : Ident → IdentVal) (i : Ident) :
+  Expr.eval ctx i = (ctx i).get none := rfl
 
 
 /-- Pretty print repr of indices; ignores [] (scalar), represents only
@@ -203,28 +202,45 @@ example : Expr R := (0 : R)
 -- def idcs_repr (idcs : list string) : string :=
 -- if idcs.length = 0 then "" else "[" ++ ", ".intercalate idcs ++ "]"
 
-def expr_repr [has_repr R] : Expr R → string
+def expr_repr [has_repr R] : Expr → string
 | (Expr.lit r) := repr r
 | (Expr.ident x) := repr x
 | (Expr.access x i) := (repr x) ++ "[" ++ (expr_repr i) ++ "]"
 | (Expr.call o args) := (repr o) ++ "(" ++ ", ".intercalate (vector.of_fn (λ i, expr_repr $ args i)).to_list ++ ")"
 
-instance [has_repr R] : has_repr (Expr R) := ⟨expr_repr⟩
+instance [has_repr R] : has_repr Expr := ⟨expr_repr⟩
 -- Because ambiguous whether R or ℕ
 -- instance : has_zero (Expr R) := ⟨Expr.lit 0⟩
 -- instance : has_one (Expr R) := ⟨Expr.lit 1⟩
 
-variable (R)
+parameter (R)
+structure LoopBound :=
+(frame : finset Ident)
+(to_fun : (Ident → IdentVal) → ℕ)
+(has_frame : function.has_frame to_fun frame)
+
+parameter {R}
+instance : has_coe_to_fun LoopBound (λ _, (Ident → IdentVal) → ℕ) :=
+⟨LoopBound.to_fun⟩
+
+@[simp] lemma to_fun_eq_coe (f : LoopBound) (ctx : Ident → IdentVal) : f.to_fun = ⇑f := rfl
+
+@[simp] lemma to_fun_apply (frame : finset Ident) (to_fun : (Ident → IdentVal) → ℕ) (h) (ctx : Ident → IdentVal) :
+  (LoopBound.mk frame to_fun h) ctx = to_fun ctx := rfl
+
+theorem LoopBound.frame_sound (f : LoopBound) {ctx₀ ctx₁ : Ident → IdentVal} (h : ∀ v ∈ f.frame, ctx₀ v = ctx₁ v) :
+  f ctx₀ = f ctx₁ := function.has_frame_iff.mp f.has_frame h
+
+parameter (R)
 inductive Prog
 | skip : Prog
-| store (dst : Ident) (ind : option (Expr R)) (val : Expr R)
+| store (dst : Ident) (ind : option Expr) (val : Expr)
 | seq (a : Prog) (b : Prog)
-| branch (cond : Expr R) (a : Prog) (b : Prog)
-| loop (n : Expr R) (b : Prog)
+| branch (cond : Expr) (a : Prog) (b : Prog)
+| loop (n : LoopBound) (b : Prog)
 
-variable {R}
-
-def prog_repr [has_repr R] : Prog R → list string
+parameter {R}
+def prog_repr [has_repr R] : Prog → list string
 | Prog.skip := [";"]
 | (Prog.store dst ind val) := [(repr dst) ++ (ind.elim "" (λ i, "[" ++ repr i ++ "]")) ++ " := " ++ (repr val) ++ ";"]
 | (Prog.seq a b) := (prog_repr a) ++ (prog_repr b)
@@ -232,43 +248,43 @@ def prog_repr [has_repr R] : Prog R → list string
     ++ (prog_repr a).map (λ s, "  " ++ s)
     ++ ["else"]
     ++ (prog_repr b).map (λ s, "  " ++ s)
-| (Prog.loop n b) := ["for at most " ++ (repr n) ++ " times"]
+| (Prog.loop n b) := ["for at most some bounded # of times"]
     ++ (prog_repr b).map (λ s, "  " ++ s)
 
-instance [has_repr R] : has_to_string (Prog R) := ⟨λ p, "\n".intercalate (prog_repr p)⟩
+instance [has_repr R] : has_to_string Prog := ⟨λ p, "\n".intercalate (prog_repr p)⟩
 
 
 
-def Prog.eval : Prog R → (Ident → IdentVal R) → (Ident → IdentVal R)
+def Prog.eval : Prog → (Ident → IdentVal) → (Ident → IdentVal)
 | Prog.skip ctx := ctx
-| (Prog.store dst ind val) ctx := function.update ctx dst ((ctx dst).update (ind.map (λ i : Expr R, (i.eval ctx).to_nat)) (val.eval ctx))
+| (Prog.store dst ind val) ctx := function.update ctx dst ((ctx dst).update (ind.map (λ i : Expr, (i.eval ctx).to_nat)) (val.eval ctx))
 | (Prog.seq a b) ctx := b.eval (a.eval ctx)
 | (Prog.branch cond a b) ctx := if 0 < (Expr.eval ctx cond).to_nat then a.eval ctx else b.eval ctx
-| (Prog.loop n b) ctx := (nat.iterate b.eval (Expr.eval ctx n).to_nat) ctx
+| (Prog.loop n b) ctx := (nat.iterate b.eval (n ctx)) ctx
 
 def alist.ilookup {α β : Type*} [decidable_eq α] [inhabited β] (s : alist (λ _ : α, β)) (a : α) : β :=
 (s.lookup a).iget
 
 -- Faster version of eval
 -- TODO: which one should be the "main" one
-def Prog.eval' : Prog R → (alist (λ _ : Ident, IdentVal R)) → (alist (λ _ : Ident, IdentVal R))
+def Prog.eval' : Prog → (alist (λ _ : Ident, IdentVal)) → (alist (λ _ : Ident, IdentVal))
 | Prog.skip ctx := ctx
-| (Prog.store dst ind val) ctx := ctx.insert dst ((ctx.ilookup dst).update (ind.map (λ i : Expr R, (i.eval ctx.ilookup).to_nat)) (val.eval ctx.ilookup))
+| (Prog.store dst ind val) ctx := ctx.insert dst ((ctx.ilookup dst).update (ind.map (λ i : Expr, (i.eval ctx.ilookup).to_nat)) (val.eval ctx.ilookup))
 | (Prog.seq a b) ctx := b.eval' (a.eval' ctx)
 | (Prog.branch cond a b) ctx := if 0 < (cond.eval ctx.ilookup).to_nat then a.eval' ctx else b.eval' ctx
-| (Prog.loop n b) ctx := (nat.iterate b.eval' (n.eval ctx.ilookup).to_nat) ctx
+| (Prog.loop n b) ctx := (nat.iterate b.eval' (n ctx.ilookup)) ctx
 
 section frame
 
 @[simp]
-def Expr.frame : Expr R → finset Ident
+def Expr.frame : Expr → finset Ident
 | (Expr.lit r) := ∅
 | (Expr.ident i) := {i}
 | (Expr.access x n) := insert x n.frame
 | (Expr.call o args) := finset.bUnion finset.univ (λ i, (args i).frame)
 
-/-- The evaluation of an Expr dependso only on the values in its frame -/
-theorem frame_sound_Expr {e : Expr R} {ctx₀ ctx₁ : Ident → IdentVal R}
+/-- The evaluation of an Expr depends only on the values in its frame -/
+theorem frame_sound_Expr {e : Expr} {ctx₀ ctx₁ : Ident → IdentVal}
   (h : ∀ v ∈ e.frame, ctx₀ v = ctx₁ v) : e.eval ctx₀ = e.eval ctx₁ :=
 begin
   induction e,
@@ -279,8 +295,11 @@ begin
   { simp, congr, ext i, apply ih, refine (λ v hv, h v _), simp, refine ⟨_, hv⟩, }
 end
 
+theorem Expr.has_frame (e : Expr) : function.has_frame (λ ctx, e.eval ctx : (Ident → IdentVal) → ExprVal) e.frame :=
+by { rw function.has_frame_iff, intros c₁ c₂, apply frame_sound_Expr, }
+
 @[simp]
-def Prog.frame : Prog R → finset Ident
+def Prog.frame : Prog → finset Ident
 | Prog.skip := ∅
 | (Prog.store dst none val) := insert dst val.frame
 | (Prog.store dst (some ind) val) := insert dst (ind.frame ∪ val.frame)
@@ -289,7 +308,7 @@ def Prog.frame : Prog R → finset Ident
 | (Prog.loop n b) := n.frame ∪ b.frame
 
 /-- Ident's not in the frame remain unchanged -/
-theorem not_mem_Prog_frame {p : Prog R} {s} (hs : s ∉ p.frame) (ctx : Ident → IdentVal R) :
+theorem not_mem_Prog_frame {p : Prog} {s} (hs : s ∉ p.frame) (ctx : Ident → IdentVal) :
   p.eval ctx s = ctx s :=
 begin
   induction p generalizing ctx,
@@ -305,14 +324,14 @@ begin
     simp [Prog.eval], split_ifs, exacts [ih₁ hs.2.1 _, ih₂ hs.2.2 _], },
   case Prog.loop : n b ih
   { simp [Prog.eval],
-    generalize : (n.eval ctx).to_nat = n',
+    generalize : n ctx = n',
     induction n' with n' ihn', { refl, },
     simp [function.iterate_succ_apply'],
     rwa ih, simp [decidable.not_or_iff_and_not] at hs, exact hs.2, }
 end
 
 /-- If two contexts agree on a set S ⊇ p.frame, then they agree after the evaluation as well. -/
-theorem frame_sound_Prog {p : Prog R} {ctx₀ ctx₁ : Ident → IdentVal R} {S : finset Ident} (hS : p.frame ⊆ S)
+theorem frame_sound_Prog {p : Prog} {ctx₀ ctx₁ : Ident → IdentVal} {S : finset Ident} (hS : p.frame ⊆ S)
   (h : ∀ v ∈ S, ctx₀ v = ctx₁ v) {s} (hs : s ∈ S) : p.eval ctx₀ s = p.eval ctx₁ s :=
 begin
   induction p generalizing ctx₀ ctx₁ s,
@@ -334,26 +353,186 @@ begin
     { exact ih₁ (finset.union_subset_left (finset.union_subset_right hS)) h hs, },
     exact ih₂ (finset.union_subset_right (finset.union_subset_right hS)) h hs, },
   case Prog.loop : n b ih
-  { have : n.eval ctx₀ = n.eval ctx₁,
-    { apply frame_sound_Expr, refine λ v hv, h v _, simp [finset.subset_iff] at hS, exact hS (or.inl hv), },
+  { have : n ctx₀ = n ctx₁,
+    { apply LoopBound.frame_sound, refine λ v hv, h v _, simp [finset.subset_iff] at hS, exact hS (or.inl hv), },
     simp [Prog.eval, this],
-    generalize : (n.eval ctx₁).to_nat = n',
+    generalize : n ctx₁ = n',
     induction n' with n' ihn generalizing s, { exact h _ hs, },
     simp [function.iterate_succ_apply'], 
     refine ih _ @ihn hs, simp at hS, exact finset.union_subset_right hS, }
 end
 
-example {β} [decidable_eq β] (s₁ s₂ S : finset β) : s₁ ∪ s₂ ⊆ S → s₁ ⊆ S  := by refine finset.union_subset_left
+def Expr.to_loop_bound (e : Expr) : LoopBound :=
+{ frame := e.frame,
+  to_fun := λ ctx, (e.eval ctx).to_nat,
+  has_frame := (Expr.has_frame e).postcomp _ }
+
+@[simp] lemma Expr.to_loop_bound_to_fun (e : Expr) (ctx : Ident → IdentVal) : e.to_loop_bound ctx = (e.eval ctx).to_nat :=
+by simp [Expr.to_loop_bound]
+
+@[simp]
+def Ident.get_num : Ident → ℕ
+| (Ident.num n) := n
+| _ := 0
+
+def fresh (S : finset Ident) : Ident :=
+Ident.num $ (finset.image (λ i : Ident, i.get_num) S).max.iget + 1
+
+theorem not_fresh_mem (S : finset Ident) : fresh S ∉ S :=
+begin
+  simp only [fresh],
+  cases hn : (finset.image (λ i : Ident, i.get_num) S).max,
+  { rw [finset.max_eq_none, finset.image_eq_empty] at hn, subst hn, exact finset.not_mem_empty _, },
+  intro h,
+  simpa using finset.le_max_of_mem (finset.mem_image_of_mem (λ i : Ident, i.get_num) h) hn,
+end
 
 end frame
 
-infixr ` <;> `:1 := Prog.seq
-notation a ` ::= `:20 c := Prog.store a none c
-notation a ` ⟬ `:9000 i ` ⟭ ` ` ::= `:20 c := Prog.store a (some i) c
-notation x ` ⟬ `:9000 i ` ⟭ ` := Expr.access x i 
+local infixr ` <;> `:1 := Prog.seq
+local notation a ` ::= `:20 c := Prog.store a none c
+local notation a ` ⟬ `:9000 i ` ⟭ ` ` ::= `:20 c := Prog.store a (some i) c
+local notation x ` ⟬ `:9000 i ` ⟭ ` := Expr.access x i 
 
--- 
-section example_prog
+parameter (R)
+structure BoundedStreamGen (ι α : Type) :=
+(current : ι)
+(value : α)
+(ready : Expr)
+(next : Prog)
+(valid : Expr)
+(bound : Expr)
+(initialize : Prog)
+
+parameter {R}
+@[ext]
+theorem BoundedStreamGen.ext {ι α} {x y : BoundedStreamGen ι α} (h₀ : x.current = y.current)
+  (h₁ : x.value = y.value) (h₂ : x.ready = y.ready) (h₃ : x.next = y.next) (h₄ : x.valid = y.valid)
+  (h₅ : x.bound = y.bound) (h₆ : x.initialize = y.initialize) : x = y :=
+by { cases x, cases y, dsimp only at *, subst_vars, }
+
+variables {ι α : Type}
+
+section functorality
+
+@[simps]
+instance : bifunctor BoundedStreamGen :=
+{ bimap := λ _ _ _ _ i v g, { g with value := v g.value, current := i g.current } }
+
+instance : is_lawful_bifunctor BoundedStreamGen :=
+{ id_bimap := λ _ _ g, by ext; simp [bimap],
+  bimap_bimap := λ _ _ _ _ _ _ i i' v v' g, by ext; simp [bimap] }
+
+infixr ` <$₁> `:1 := bifunctor.fst
+infixr ` <$₂> `:1 := bifunctor.snd
+
+-- TODO: find a better way
+variables {ι' α' : Type} (f : ι → ι') (g : α → α') (s : BoundedStreamGen ι α)
+@[simp] lemma BSG_fst_value : (f <$₁> s).value = s.value := rfl 
+@[simp] lemma BSG_fst_ready : (f <$₁> s).ready = s.ready := rfl
+@[simp] lemma BSG_fst_next : (f <$₁> s).next = s.next := rfl
+@[simp] lemma BSG_fst_valid : (f <$₁> s).valid = s.valid := rfl
+@[simp] lemma BSG_fst_bound : (f <$₁> s).bound = s.bound := rfl
+@[simp] lemma BSG_fst_init : (f <$₁> s).initialize = s.initialize := rfl
+@[simp] lemma BSG_snd_current : (g <$₂> s).current = s.current := rfl 
+@[simp] lemma BSG_snd_ready : (g <$₂> s).ready = s.ready := rfl
+@[simp] lemma BSG_snd_next : (g <$₂> s).next = s.next := rfl
+@[simp] lemma BSG_snd_valid : (g <$₂> s).valid = s.valid := rfl
+@[simp] lemma BSG_snd_bound : (g <$₂> s).bound = s.bound := rfl
+@[simp] lemma BSG_snd_init : (g <$₂> s).initialize = s.initialize := rfl
+
+@[simp] lemma BSG_fst_current : (f <$₁> s).current = f s.current := rfl
+@[simp] lemma BSG_snd_value : (g <$₂> s).value = g s.value := rfl
+
+attribute [functor_norm] bifunctor.fst_snd bifunctor.snd_fst
+
+end functorality
+
+@[pattern]
+def Prog.if1 (cond : Expr) (b : Prog) := Prog.branch cond b Prog.skip
+
+def BoundedStreamGen.compile (g : BoundedStreamGen unit Prog) : Prog :=
+g.initialize <;>
+Ident.reserved_break ::= (0 : ℕ) <;>
+Prog.loop (Expr.to_loop_bound g.bound) $
+  Prog.if1 (Expr.call Op.not ![Ident.reserved_break]) $
+    Prog.if1 g.ready g.value <;>
+    Prog.branch g.valid g.next (Ident.reserved_break ::= (1 : ℕ))
+
+parameter (R)
+/-- Indicates that things of type α (which typically involve Expr R)'s can eval
+  to things of type β given a context ctx : Ident → IdentVal R -/
+class StreamEval (α β: Type) :=
+(eval : α → (Ident → IdentVal) → β)
+
+/-- An Compileable.compile (f, e) indicates that f describes how to compile e to a program -/
+class Compileable (α β : Type) :=
+(compile : α → β → Prog)
+
+parameter {R}
+-- This is ind_eval, but we need to support recursion so we extract it specifically
+-- Mathlib's lack of computability bites here;
+-- since finsupp is noncomputable (this is actually a controversial-ish decision from what I gather from the Zulip)
+-- it poisons "eval_stream"
+-- We only use +, finsupp.single and finsupp.zero (zero is computable), so maybe a TODO is a computable implementation
+@[simp]
+noncomputable def eval_stream {ι β : Type} [add_zero_class β] :
+  ℕ → (Ident → IdentVal) → (BoundedStreamGen ((Ident → IdentVal) → ι) ((Ident → IdentVal) → β)) → (ι →₀ β)
+| 0 _ _ := 0
+| (n+1) ctx s :=
+if (s.valid.eval ctx).to_nat = 1 then
+  (if (s.ready.eval ctx).to_nat = 1 then finsupp.single (s.current ctx) (s.value ctx) else 0)
+    + (eval_stream n (s.next.eval ctx) s)
+else 0
+
+instance base_eval : StreamEval Expr ExprVal :=
+⟨λ e ctx, e.eval ctx⟩
+
+instance base_eval_nat : StreamEval Expr ℕ :=
+⟨λ e ctx, (e.eval ctx).to_nat⟩
+
+instance base_eval_R : StreamEval Expr R :=
+⟨λ e ctx, (e.eval ctx).to_r⟩
+
+instance refl_eval {α : Type} : StreamEval α α := ⟨λ x _, x⟩
+
+noncomputable instance ind_eval {ι ι' α β : Type} [StreamEval ι ι'] [StreamEval α β] [add_zero_class β] :
+  StreamEval (BoundedStreamGen ι α) (ι' →₀ β) :=
+{ eval := λ s ctx, eval_stream (s.bound.eval ctx).to_nat (s.initialize.eval ctx) 
+  (StreamEval.eval <$₁> StreamEval.eval <$₂> s) }
+
+/- Convenience instance for `unit` so we don't have to write `unit → R` and can directly go to R
+TODO: Remove? -/
+noncomputable instance unit_eval {α β : Type} [StreamEval α β] [add_zero_class β] :
+  StreamEval (BoundedStreamGen unit α) β :=
+{ eval := λ s ctx, (StreamEval.eval s ctx : unit →₀ β) () }
+
+instance base_compile : Compileable (Expr → Prog) Expr := 
+⟨λ c e, c e⟩
+
+section laws
+-- Law 1: eval frame should be frame
+
+-- Law 2: eval for bound steps should make invalid
+
+end laws
+
+section variable_state
+
+structure WithFrame (α : Type) : Type :=
+(val : α)
+(frame : finset Ident)
+
+instance WithFrame_coe {α : Type} : has_coe (WithFrame α) α := ⟨WithFrame.val⟩ 
+
+def WithFrame.is_sound (β : Type) [StreamEval α β] (x : WithFrame α) : Prop :=
+function.has_frame (StreamEval.eval (x : α) : (Ident → IdentVal) → β) x.frame
+
+def WithFrame.fresh {β : Type} (x : WithFrame α) (f : Ident → β) : WithFrame β :=
+⟨f (fresh x.frame), insert (fresh x.frame) x.frame⟩
+
+end variable_state
+
 namespace vars
 
 abbreviation x := Ident.of "x"
@@ -366,233 +545,53 @@ abbreviation output := Ident.of "output"
 
 end vars
 
-open Expr Prog vars
-
-def pow_prog : Prog ℤ :=
-z ::= (1 : ℤ) <;>
-loop y (z ::= x ⟪*⟫ z)
-
-def pow_prog_input (i : Ident) : IdentVal ℤ :=
-  if i = x then IdentVal.base (ExprVal.rval 3)
-  else if i = y then IdentVal.base (ExprVal.nat 4)
-  else arbitrary _
-
-def arr_prog : Prog ℤ :=
-s ::= (0 : ℤ) <;>
-i ::= (0 : ℕ) <;>
-loop y $
-  s ::= s ⟪+⟫ x⟬i⟭ <;>
-  i ::= i ⟪+⟫ (1 : ℕ)
-
-def arr_prog_input (i : Ident) : IdentVal ℤ :=
-  if i = x then IdentVal.arr [ExprVal.rval 30, ExprVal.rval (-1), ExprVal.rval 4]
-  else if i = y then IdentVal.base (ExprVal.nat 3)
-  else arbitrary _
-
-def range_sum : Prog ℤ :=
-s ::= (0 : ℤ) <;>
-i ::= (0 : ℕ) <;>
-loop (500 : ℕ) $
-  s ::= s ⟪+⟫ (Expr.call Op.cast_r ![i]) <;>
-  i ::= i ⟪+⟫ (1 : ℕ)
-
-
-end example_prog
-
-variable (R)
-@[ext]
-structure BoundedStreamGen (ι α : Type) :=
-(current : ι)
-(value : α)
-(ready : Expr R)
-(next : Prog R)
-(valid : Expr R)
-(bound : Expr R)
-(reset : Prog R)
-(initialize : Prog R)
-
-variables {ι α : Type} {R}
-
-section functorality
-
-@[simps]
-instance : bifunctor (BoundedStreamGen R) :=
-{ bimap := λ _ _ _ _ i v g, { g with value := v g.value, current := i g.current } }
-
-instance : is_lawful_bifunctor (BoundedStreamGen R) :=
-{ id_bimap := λ _ _ g, by ext; simp [bimap],
-  bimap_bimap := λ _ _ _ _ _ _ i i' v v' g, by ext; simp [bimap] }
-
-infixr ` <$₁> `:1 := bifunctor.fst
-infixr ` <$₂> `:1 := bifunctor.snd
-
--- TODO: find a better way
-variables {ι' α' : Type} (f : ι → ι') (g : α → α') (s : BoundedStreamGen R ι α)
-@[simp] lemma BSG_fst_value : (f <$₁> s).value = s.value := rfl 
-@[simp] lemma BSG_fst_ready : (f <$₁> s).ready = s.ready := rfl
-@[simp] lemma BSG_fst_next : (f <$₁> s).next = s.next := rfl
-@[simp] lemma BSG_fst_valid : (f <$₁> s).valid = s.valid := rfl
-@[simp] lemma BSG_fst_bound : (f <$₁> s).bound = s.bound := rfl
-@[simp] lemma BSG_fst_reset : (f <$₁> s).reset = s.reset := rfl
-@[simp] lemma BSG_fst_init : (f <$₁> s).initialize = s.initialize := rfl
-@[simp] lemma BSG_snd_current : (g <$₂> s).current = s.current := rfl 
-@[simp] lemma BSG_snd_ready : (g <$₂> s).ready = s.ready := rfl
-@[simp] lemma BSG_snd_next : (g <$₂> s).next = s.next := rfl
-@[simp] lemma BSG_snd_valid : (g <$₂> s).valid = s.valid := rfl
-@[simp] lemma BSG_snd_bound : (g <$₂> s).bound = s.bound := rfl
-@[simp] lemma BSG_snd_reset : (g <$₂> s).reset = s.reset := rfl
-@[simp] lemma BSG_snd_init : (g <$₂> s).initialize = s.initialize := rfl
-
-@[simp] lemma BSG_fst_current : (f <$₁> s).current = f s.current := rfl
-@[simp] lemma BSG_snd_value : (g <$₂> s).value = g s.value := rfl
-
-attribute [functor_norm] bifunctor.fst_snd bifunctor.snd_fst
-
-end functorality
-
-@[pattern]
-def Prog.if1 (cond : Expr R) (b : Prog R) := Prog.branch cond b Prog.skip
-
-def BoundedStreamGen.compile (g : BoundedStreamGen R unit (Prog R)) : Prog R :=
-g.initialize <;>
-Ident.reserved_break ::= (0 : ℕ) <;>
-Prog.loop g.bound $
-  Prog.if1 (Expr.call Op.not ![Ident.reserved_break]) $
-    Prog.if1 g.ready g.value <;>
-    Prog.branch g.valid g.next (Ident.reserved_break ::= (1 : ℕ))
-
-variable (R)
-
-/-- Indicates that things of type α (which typically involve Expr R)'s can eval
-  to things of type β given a context ctx : Ident → IdentVal R -/
-class StreamEval (α β: Type) :=
-(eval : (Ident → IdentVal R) → α → β)
-
-/-- An Compileable.compile (f, e) indicates that f describes how to compile e to a program -/
-class Compileable (α β : Type) :=
-(compile : α → β → Prog R)
-
-variable {R}
--- This is ind_eval, but we need to support recursion so we extract it specifically
--- Mathlib's lack of computability bites here;
--- since finsupp is noncomputable (this is actually a controversial-ish decision from what I gather from the Zulip)
--- it poisons "eval_stream"
--- We only use +, finsupp.single and finsupp.zero (zero is computable), so maybe a TODO is a computable implementation
-@[simp]
-noncomputable def eval_stream {ι β : Type} [add_zero_class β] :
-  ℕ → (Ident → IdentVal R) → (BoundedStreamGen R ((Ident → IdentVal R) → ι) ((Ident → IdentVal R) → β)) → (ι →₀ β)
-| 0 _ _ := 0
-| (n+1) ctx s :=
-if (s.valid.eval ctx).to_nat = 1 then
-  (if (s.ready.eval ctx).to_nat = 1 then finsupp.single (s.current ctx) (s.value ctx) else 0)
-    + (eval_stream n (s.next.eval ctx) s)
-else 0
-
-instance base_eval : StreamEval R (Expr R) (ExprVal R) :=
-⟨Expr.eval⟩
-
-instance base_eval_nat : StreamEval R (Expr R) ℕ :=
-⟨λ ctx e, (e.eval ctx).to_nat⟩
-
-instance base_eval_R : StreamEval R (Expr R) R :=
-⟨λ ctx e, (e.eval ctx).to_r⟩
-
-instance refl_eval {α : Type} : StreamEval R α α := ⟨λ _, id⟩
-
-noncomputable instance ind_eval {ι ι' α β : Type} [StreamEval R ι ι'] [StreamEval R α β] [add_zero_class β] :
-  StreamEval R (BoundedStreamGen R ι α) (ι' →₀ β) :=
-{ eval := λ ctx s, eval_stream (s.bound.eval ctx).to_nat (s.initialize.eval ctx) 
-  ((λ i ctx', StreamEval.eval ctx' i) <$₁> (λ i ctx', StreamEval.eval ctx' i) <$₂> s) }
-
-/- Convenience instance for `unit` so we don't have to write `unit → R` and can directly go to R
-TODO: Remove? -/
-noncomputable instance unit_eval {α β : Type} [StreamEval R α β] [add_zero_class β] :
-  StreamEval R (BoundedStreamGen R unit α) β :=
-{ eval := λ ctx s, (StreamEval.eval ctx s : unit →₀ β) () }
-
-instance base_compile : Compileable R (Expr R → Prog R) (Expr R) := 
-⟨λ c e, c e⟩
-
-section variable_counter
-
-structure MState :=
-(counter : ℕ)
-
-@[reducible] def M := state MState
-def M.fresh : M Ident :=
-{ run := λ σ, (Ident.num σ.counter, ⟨σ.counter + 1⟩) }
-
-def M.get {σ} (x : M σ) : σ := (x.run ⟨0⟩).1
-def M.getn {σ} (n : ℕ) (x : M σ) : σ := (x.run ⟨n⟩).1
-
-def MRespects {β : Type} [StreamEval R α β] (x : M α) : Prop :=
-∀ (ctx₁ ctx₂ : Ident → IdentVal R),
-  (∀ n < (x.run ⟨0⟩).2.counter, ctx₁ (Ident.num n) = ctx₂ (Ident.num n)) →
-    (StreamEval.eval ctx₁ (M.get x) : β) = StreamEval.eval ctx₂ (M.get x)
-
-@[simp] lemma get_fresh_bind {α : Type} (f : Ident → M α) :
-  M.get (M.fresh >>= f) = M.getn 1 (f (Ident.num 0)) := rfl
-  
-@[simp] lemma getn_fresh_bind {α : Type} (n : ℕ) (f : Ident → M α) :
-  M.getn n (M.fresh >>= f) = M.getn (n+1) (f (Ident.num n)) := rfl
-
-@[simp] lemma get_fresh_pure {α} (f : α) : M.get (return f) = f := rfl
-
-@[simp] lemma getn_fresh_pure {α : Type} (n : ℕ) (f : α) :
-  M.getn n (return f) = f := rfl
-
-end variable_counter
-
 section singleton
 
-def BoundedStreamGen.singleton (a : α) : M (BoundedStreamGen R unit α) :=
-do i ← M.fresh,
-  return
+def BoundedStreamGen.singleton (a : WithFrame α) : WithFrame (BoundedStreamGen unit α) :=
+a.fresh $ λ i,
 { current := (),
   value := a,
   ready := (1 : ℕ),
   valid := i ⟪<⟫ (1 : ℕ),
   bound := (1 : ℕ),
   next := i ::= (1 : ℕ),
-  reset := Prog.skip,
   initialize := i ::= (0 : ℕ) }
-
-theorem singleton_spec {β : Type} [add_zero_class β] [StreamEval R α β] (ctx : Ident → IdentVal R) (a : α) :
-  (StreamEval.eval ctx (M.get $ BoundedStreamGen.singleton a : BoundedStreamGen R unit α) : β) = StreamEval.eval ctx a :=
-begin
-  simp [StreamEval.eval, Prog.eval, BoundedStreamGen.singleton], sorry,
-end
+-- theorem singleton_spec {β : Type} [add_zero_class β] [StreamEval α β] (ctx : Ident → IdentVal R) (a : α) :
+--   (StreamEval.eval ctx (M.get $ BoundedStreamGen.singleton a : BoundedStreamGen R unit α) : β) = StreamEval.eval ctx a :=
+-- begin
+--   simp [StreamEval.eval, Prog.eval, BoundedStreamGen.singleton], sorry,
+-- end
 
 end singleton
 
-def BoundedStreamGen.expr_to_prog (inp : BoundedStreamGen R unit (Expr R)) : BoundedStreamGen R unit (Prog R) :=
+
+
+def BoundedStreamGen.expr_to_prog (inp : BoundedStreamGen unit Expr) : BoundedStreamGen unit Prog :=
 { current := (),
   value := vars.output ::= vars.output ⟪+⟫ inp.value,
   ready := inp.ready,
   next := inp.next,
   valid := inp.valid,
   bound := inp.bound,
-  reset := inp.reset,
   initialize := inp.initialize <;> vars.output ::= (0 : R) }
 
-section example_singleton
+-- section example_singleton
 
-def test : BoundedStreamGen ℤ unit (Expr ℤ) := M.get (BoundedStreamGen.singleton (10 : ℤ))
+-- def test : BoundedStreamGen ℤ unit (Expr ℤ) := M.get (BoundedStreamGen.singleton (10 : ℤ))
 
-lemma test_eval : (StreamEval.eval (λ _, arbitrary (IdentVal ℤ)) test : ℤ) = 10 :=
-by { simp [StreamEval.eval, test, Prog.eval, BoundedStreamGen.singleton], }
+-- lemma test_eval : (StreamEval.eval (λ _, arbitrary (IdentVal ℤ)) test : ℤ) = 10 :=
+-- by { simp [StreamEval.eval, test, Prog.eval, BoundedStreamGen.singleton], }
 
-end example_singleton
+-- end example_singleton
 
 section range
 
-def range (n : Expr R) (var : Ident) : BoundedStreamGen R (Expr R) (Expr R) :=
+def range (n : Expr) (var : Ident) : BoundedStreamGen Expr Expr :=
 { current := var,
   value := Expr.call Op.cast_r ![var],
   ready := var ⟪<⟫ n,
   valid := var ⟪<⟫ n,
   next := var ::= var ⟪+⟫ (1 : ℕ),
-  reset := var ::= (0 : ℕ),
   bound := n,
   initialize := var ::= (0 : ℕ), }
 
@@ -602,11 +601,11 @@ end range
 
 section contract
 
-def contract (g : BoundedStreamGen R ι α) : BoundedStreamGen R unit α :=
+def contract (g : BoundedStreamGen ι α) : BoundedStreamGen unit α :=
 (λ _, ()) <$₁> g
 
-lemma contract_aux [add_comm_monoid α] (n : ℕ) (ctx : Ident → IdentVal R) 
-  (g : BoundedStreamGen R ((Ident → IdentVal R) → ι) ((Ident → IdentVal R) → α)) :
+lemma contract_aux [add_comm_monoid α] (n : ℕ) (ctx : Ident → IdentVal) 
+  (g : BoundedStreamGen ((Ident → IdentVal) → ι) ((Ident → IdentVal) → α)) :
   (eval_stream n ctx ((λ _ _, ()) <$₁> g)) () = (eval_stream n ctx g).sum_range :=
 begin
   induction n with n ih generalizing ctx, { simp, },
@@ -617,13 +616,12 @@ begin
   refl, -- Invalid, both are 0
 end
 
-theorem contract_spec {β ι' : Type} [add_comm_monoid β] [StreamEval R α β] [StreamEval R ι ι']
-  (s : BoundedStreamGen R ι α) (ctx : Ident → IdentVal R) :
-  StreamEval.eval ctx (contract s) = (StreamEval.eval ctx s : ι' →₀ β).sum_range :=
+theorem contract_spec {β ι' : Type} [add_comm_monoid β] [StreamEval α β] [StreamEval ι ι']
+  (s : BoundedStreamGen ι α) (ctx : Ident → IdentVal) :
+  StreamEval.eval (contract s) ctx = (StreamEval.eval s ctx : ι' →₀ β).sum_range :=
 by simpa [StreamEval.eval, contract, bifunctor.fst] with functor_norm
 using contract_aux (s.bound.eval ctx).to_nat (s.initialize.eval ctx)
-      ((λ i ctx', StreamEval.eval ctx' i) <$₁>
-        (λ i ctx', StreamEval.eval ctx' i) <$₂> s)
+      (StreamEval.eval <$₁> StreamEval.eval <$₂> s)
 
 end contract
 
@@ -631,37 +629,35 @@ section repeat
 
 end repeat
 
-def flatten {ι₁ ι₂ α : Type} (outer : BoundedStreamGen R ι₁ (BoundedStreamGen R ι₂ α)) :
-  BoundedStreamGen R (ι₁ × ι₂) α :=
+def flatten {ι₁ ι₂ α : Type} (outer : BoundedStreamGen ι₁ (BoundedStreamGen ι₂ α)) :
+  BoundedStreamGen (ι₁ × ι₂) α :=
 let inner := outer.value in
 { current := (outer.current, inner.current),
   value := inner.value,
   ready := outer.ready ⟪&&⟫ inner.ready,
-  next := let next_outer := outer.next <;> inner.reset in
+  next := let next_outer := outer.next <;> inner.initialize in
   Prog.branch outer.ready 
     (Prog.branch inner.valid inner.next next_outer) 
     next_outer,
   valid := outer.valid,
   bound := outer.bound ⟪*⟫ inner.bound, -- TODO: fix
-  reset := outer.reset <;> inner.reset, -- TODO: fix
   initialize := outer.initialize <;> inner.initialize }
 
-def test₂ : BoundedStreamGen ℤ (Expr ℤ) (Expr ℤ) := range (40 : ℕ) vars.x
+-- def test₂ : BoundedStreamGen ℤ (Expr ℤ) (Expr ℤ) := range (40 : ℕ) vars.x
 -- #eval trace_val $ to_string $ (contract test₂).expr_to_prog.compile
 -- #eval (((contract test₂).expr_to_prog.compile.eval' ∅).ilookup vars.output).get none
 
-def externVec (len : Expr R) (inp : Ident) (inp_idx : Ident) : BoundedStreamGen R (Expr R) (Expr R) :=
+def externVec (len : Expr) (inp : Ident) (inp_idx : Ident) : BoundedStreamGen Expr Expr :=
 { current := inp_idx,
   value := inp⟬ inp_idx ⟭,
   ready := inp_idx ⟪<⟫ len,
   next := inp_idx ::= inp_idx ⟪+⟫ (1 : ℕ),
   valid := inp_idx ⟪<⟫ len,
   bound := len,
-  reset := inp_idx ::= (0 : ℕ),
   initialize := inp_idx ::= (0 : ℕ) }
 
-def externCSRMat (l₁ l₂ : Expr R) (rows cols data : Ident) (i j k : Ident) :
-  BoundedStreamGen R (Expr R × Expr R) (Expr R) :=
+def externCSRMat (l₁ l₂ : Expr) (rows cols data : Ident) (i j k : Ident) :
+  BoundedStreamGen (Expr × Expr) Expr :=
 { current := (i, cols⟬j⟭),
   value := data⟬k⟭,
   ready := j ⟪<⟫ rows⟬i ⟪+⟫ (1 : ℕ)⟭,
@@ -672,10 +668,59 @@ def externCSRMat (l₁ l₂ : Expr R) (rows cols data : Ident) (i j k : Ident) :
       (i ::= i ⟪+⟫ (1 : ℕ)),
   valid := i ⟪<⟫ l₁,
   bound := l₁ ⟪*⟫ l₂ ,
-  reset := i ::= (0 : ℕ) <;> j ::= (0 : ℕ) <;> k ::= (0 : ℕ),
-  initialize := Prog.skip }
+  initialize := i ::= (0 : ℕ) <;> j ::= (0 : ℕ) <;> k ::= (0 : ℕ), }
 
 
-def test₃ : BoundedStreamGen ℤ (Expr ℤ) (Expr ℤ) := externVec (10 : ℕ) (Ident.of "input") (Ident.of "idx") 
+-- def test₃ : BoundedStreamGen ℤ (Expr ℤ) (Expr ℤ) := externVec (10 : ℕ) (Ident.of "input") (Ident.of "idx") 
 
 -- #eval trace_val $ to_string $ (contraction (Ident.of "acc") test₃).expr_to_prog.compile
+
+end
+
+-- Examples
+
+-- section example_prog
+-- namespace vars
+
+-- abbreviation x := Ident.of "x"
+-- abbreviation y := Ident.of "y"
+-- abbreviation z := Ident.of "z"
+-- abbreviation s := Ident.of "s"
+-- abbreviation i := Ident.of "i"
+-- abbreviation acc := Ident.of "acc"
+-- abbreviation output := Ident.of "output"
+
+-- end vars
+
+-- open Expr Prog vars
+
+-- def pow_prog : Prog ℤ :=
+-- z ::= (1 : ℤ) <;>
+-- loop ⟨_, _, function.has_frame.const _ _ 4⟩ (z ::= x ⟪*⟫ z)
+
+-- def pow_prog_input (i : Ident) : IdentVal ℤ :=
+--   if i = x then IdentVal.base (ExprVal.rval 3)
+--   else if i = y then IdentVal.base (ExprVal.nat 4)
+--   else arbitrary _
+
+-- def arr_prog : Prog ℤ :=
+-- s ::= (0 : ℤ) <;>
+-- i ::= (0 : ℕ) <;>
+-- loop (Expr.to_loop_bound y) $
+--   s ::= s ⟪+⟫ x⟬i⟭ <;>
+--   i ::= i ⟪+⟫ (1 : ℕ)
+
+-- def arr_prog_input (i : Ident) : IdentVal ℤ :=
+--   if i = x then IdentVal.arr [ExprVal.rval 30, ExprVal.rval (-1), ExprVal.rval 4]
+--   else if i = y then IdentVal.base (ExprVal.nat 3)
+--   else arbitrary _
+
+-- def range_sum : Prog ℤ :=
+-- s ::= (0 : ℤ) <;>
+-- i ::= (0 : ℕ) <;>
+-- loop ⟨_, _, function.has_frame.const _ _ 500⟩ $
+--   s ::= s ⟪+⟫ (Expr.call Op.cast_r ![i]) <;>
+--   i ::= i ⟪+⟫ (1 : ℕ)
+
+
+-- end example_prog
